\title{Chapter 4, Section 4. Exercises 1, 2, and 4.}
\author{
	MTH 594, Prof. Mikael Vejdemo-Johansson \\
	Differential Geometry Independent Study \\
	\\
	Matthew Connelly \\
}
\date{\today}



\documentclass[12pt]{article}

\usepackage[top=.5in, bottom=.75in, left=1in, right=1in]{geometry}
\usepackage{amssymb}
\usepackage{amsmath}
\usepackage{graphicx}
\usepackage{subcaption}

\newcommand{\ulind}[1]
{
\noindent
\underline{#1}\\\\
\indent
}

\newcommand{\R}
{
\mathbb{R}
}

\begin{document}
\maketitle

\section*{Exercise 4.4.1}
\indent

Find the equation of the tangent plane of each of the following surface patches at the indicated points:\\

$$
(i) \ \sigma(u,v) = (u,v,u^2-v^2), \ (1,1,0)
$$
$$
(ii) \ \sigma(r,\theta) = (r \cosh \theta, r \sinh \theta,r^2), \ (1,0,1)
$$

\vspace{1cm}
\hrule
\vspace{1cm}
\noindent

\ulind{Preliminaries}

The equation of a tangent plane to a surface $z = f(x,y)$ at point $(x_0,y_0,z_0)$ is as follows:
$$
z = f_x(x_0,y_0)(x-x_0)+f_y(x_0,y_0)(y-y_0)+z_0
$$

\ulind{Solutions}
(i):\\
We are given $\sigma(u,v) = (u,v,u^2-v^2)$ and point $(1,1,0)$.\\
The partial derivatives of $\sigma$ are
$$
\sigma_u = (1,0,2u), \ \sigma_v = (0,1,-2v). 
$$
Computing $\sigma_u$ and $\sigma_v$ at $(1,1,0)$ gives
$$
\sigma_u(1,1,0) = (1,0,2), \ \ \sigma_v(1,1,0) = (0,1,-2). 
$$
Crossing these partials gives us our normal:
$$
\sigma_u \times \sigma_v = (-2,2,1)
$$
Our tangent plane will then be
$$
-2(x-1)+2(y-1)+(z)=0
$$

$$
(-2x+2)+(2y-2)+(z)=0
$$

$$
-2x+2y+z=0
$$
\\
(ii):\\
Same procedure as for (i).\\
We are given $\sigma(r,\theta) = (r \cosh \theta, r \sinh \theta,r^2)$ and point $(1,0,1)$.\\
The partial derivatives of $\sigma$ are
$$
\sigma_r(\cosh\theta, \sinh \theta,2r), \ \sigma_\theta = (r\sinh\theta,r\cosh\theta,0)
$$
From here, we'll solve for $r, \theta$:
$$1 = r\cosh\theta$$
$$0 = r\sinh\theta$$
$$1 = r^2$$

Solving the above yields $r = 1, \ \theta = 0$.\\


Finding the normal:
$$
\sigma_r \times \sigma_\theta = (-2r^2\cosh\theta,2r^2\sinh\theta,r)
$$
Using found $r$ and $\theta$ values, the normal is $(-2,0,1)$.\\
Our tangent plane is then
$$
-2(x-1)+0(y-0)+1(z-1) = 0
$$
$$
-2x+z+1 = 0
$$


\end{document}
